src/ExpManipulation.v
@@ -39,6 +39,7 @@ match e with
  | EIf e1 e2 e3 => EIf (rename ρ e1) (rename ρ e2) (rename ρ e3)
  | ECons e1 e2 => ECons (rename ρ e1) (rename ρ e2)
  | ENil => e
+ | VCons e1 e2 => VCons (rename ρ e1) (rename ρ e2)
 end.
 
 Definition Substitution := nat -> Exp + nat. (** We need to have the names for the
@@ -82,6 +83,7 @@ match base with
  | EIf e1 e2 e3 => EIf (subst ξ e1) (subst ξ e2) (subst ξ e3)
  | ECons e1 e2 => ECons (subst ξ e1) (subst ξ e2)
  | ENil => base
+ | VCons e1 e2 => VCons (subst ξ e1) (subst ξ e2)
 end.
 
 Definition scons {X : Type} (s : X) (σ : nat -> X) (x : nat) : X :=
@@ -159,6 +161,7 @@ Proof.
   * rewrite <- ren_up, <- renn_up, IHe1, IHe2, <- ren_up. auto.
   * rewrite IHe1, IHe2. auto.
   * rewrite IHe1, IHe2, IHe3. auto.
+  * now rewrite IHe1, IHe2.
   * now rewrite IHe1, IHe2.
   * constructor; auto.
   * constructor.
@@ -244,6 +247,7 @@ Proof.
   * rewrite IHe1, IHe2. auto.
   * rewrite IHe1, IHe2, IHe3. auto.
   * now rewrite IHe1, IHe2.
+  * now rewrite IHe1, IHe2.
 Qed.
 
 Notation "σ >> ξ" := (substcomp σ ξ) (at level 56, left associativity).
@@ -275,6 +279,7 @@ Proof.
   * now rewrite IHe1, IHe2.
   * now rewrite IHe1, IHe2, IHe3.
   * now rewrite IHe1, IHe2.
+  * now rewrite IHe1, IHe2.
 Qed.
 
 Theorem rename_comp :
@@ -287,6 +292,7 @@ Proof.
   * do 2 fold_upn. now rewrite IHe1, IHe2, uprenn_comp, upren_comp.
   * now rewrite IHe1, IHe2.
   * now rewrite IHe1, IHe2, IHe3.
+  * now rewrite IHe1, IHe2.
   * now rewrite IHe1, IHe2.
 Qed.
 
@@ -327,6 +333,7 @@ Proof.
   * now rewrite IHe1, IHe2.
   * now rewrite IHe1, IHe2, IHe3.
   * now rewrite IHe1, IHe2.
+  * now rewrite IHe1, IHe2.
 Qed.
 
 Lemma up_comp ξ η :
@@ -360,6 +367,7 @@ Proof.
   * do 3 fold_upn. now rewrite IHe1, IHe2, upn_comp, up_comp.
   * now rewrite IHe1, IHe2.
   * now rewrite IHe1, IHe2, IHe3.
+  * now rewrite IHe1, IHe2.
   * now rewrite IHe1, IHe2.
 Qed.
 
